First almost final version (still comp on refinement nodes to define).

paper/ITP/Below.v
@@ -1,5 +1,24 @@
+(** printing ~= $\simeq$ *)
 (* begin hide *)
-Require Import Equations.
+Require Import Equations Bvector.
+
+Equations(nocomp noeqns noind) below_vector A (P : Π n, vector A n -> Type)
+  (step : Π n (v : vector A n), Below_vector A P n v -> P n v)
+  n (v : vector A n) : Below_vector A P n v :=
+below_vector A P step O Vnil := tt ;
+below_vector A P step (S n) (Vcons a n v) :=
+  let rest := below_vector A P step n v in
+    (step n v rest, rest).
+
+Definition rec_vector A (P : Π n, vector A n -> Type) n v
+  (step : Π n (v : vector A n), Below_vector A P n v -> P n v) : P n v :=
+  step n v (below_vector A P step n v).
+
+Instance vect_Recursor A n : Recursor (vector A n) :=
+  { rec_type := λ v, Π (P : Π n, vector A n -> Type) step, P n v;
+    rec := λ v P step, rec_vector A P n v step }.
+
+Hint Unfold rec_nat rec_vector : Recursors.
 (* end hide *)
 
 Equations Below_nat (P : nat -> Type) (n : nat) : Type :=
@@ -40,7 +59,7 @@ Definition rec_nat (P : nat -> Type)
    dependent inductive object. For example, consider defining 
    [vlast]: *)
 (* begin hide *)
-Require Import Bvector.
+Transparent Below_vector.
 Hint Unfold noConfusion_nat : equations.
 (* end hide *)
 
@@ -54,9 +73,8 @@ vlast A ?(S n) (Vcons a ?(S n) v) := vlast v.
    the splitting tree), we apply the recursor for the 
    type of [v], after having properly generalized it. The recursion hypothesis 
    is hence of the form: [[
-   Below_vector A (λ (n' : nat) (v' : vector A n') =>
-     Π (n : nat) (v : vector A (S n)),
-     n' = S n -> v' ~= v -> vlast_comp v) n v ]]
+   Below_vector A (λ (n' : nat) (v' : vector A n'),
+     Π n (v : vector A (S n)), n' = S n -> v' ~= v -> vlast_comp v) n v ]]
 
    When we use non-structural recursion, recursive calls are rewritten 
    as applications of a trivial generic projection operator for the
@@ -67,8 +85,9 @@ vlast A ?(S n) (Vcons a ?(S n) v) := vlast v.
    The last argument of the projection is implicit and will be filled 
    either automatically by a proof search procedure or interactively by
    the user. When we typecheck a recursive call, the procedure will try
-   to find a satisfying [vlast_comp] object in the context, potentially 
-   simplifying [Below] hypotheses and using specialization to find it. *)
+   to find a satisfying [vlast_comp] object in the context,
+   simplifying and applying [Below_vector] hypotheses. *)
 (* begin hide *)
+Check @vlast_comp.
 (*Recursive Extraction vlast.*)
 (* end hide *)
