paper/ITP/wf.v
@@ -3,7 +3,7 @@
 Require Import Equations Relations Transitive_Closure Bvector.
 Generalizable All Variables. Set Automatic Introduction. Print clos_trans.
 Derive Subterm for vector.
-Check Acc. Check @Acc_intro.
+Check Acc. Check @Acc_intro. Definition Below : nat := 0.
 (* end hide *)
 
 (** The traditional notion of well-founded relation as found in the Coq
@@ -15,10 +15,10 @@ Inductive Acc {A} (R : A -> A -> Prop) (x : A) : Prop :=
   An element of [Acc A R x] contains a proof that any preceding element of 
   [x] by [R] (if any) is also accessible. As objects of [Acc] are inductive,
   there has to a finite proof for the accessibility of [x], hence all possible
-  chains $\cdots R~x_{i-1} x_i, R~x_i~x$ have to be finite. This corresponds 
-  (classicaly) to the descending chain condition. 
-  A relation is said to be well-founded if all elements are accessible for it. 
-   We make a class to register well founded relations: *)
+  chains $\cdots R~x_{i-1} x_i, R~x_i~x$ have to be finite. 
+  A relation is said to be well-founded if all elements of its support
+  are accessible for it. This corresponds (classicaly) to the descending 
+  chain condition. We make a class to register well founded relations: *)
 
 Class WellFounded {A : Type} (R : relation A) := wellfounded : forall a, Acc R a.
 
@@ -29,46 +29,52 @@ Definition FixWf `{WF : WellFounded A R} (P : A -> Type)
   (step : Π x : A, (Π y : A, R y x -> P y) -> P x) : Π x : A, P x.
 Proof. Admitted.
 
-(** Obviously, we can prove that the subterm relation defined
+(** Obviously, we can prove that the direct subterm relation defined
    above is well-founded. It follows by a simple induction on the object
    and inversion on the subterm proof relating the subterms and the original
-   term. However, we need to take the transitive closure of this relation 
-   to get the complete subterm relation. It is easy to show that the 
-   transitive closure of a well-founded relation is also well-founded.
+   term. We still need to take the transitive closure of this relation 
+   to get the complete subterm relation. Again it is easily shown that
+   transitive closure preserves well-foundedness.
 
+   Using this recursion scheme produces more efficient
+   programs, as only the needed recursive calls have to be computed along
+   with the corresponding proofs of the subterm relation.
+   Extraction of [FixWf] is actually a general fixpoint.
+   
    We can use the same technique as before to use this fixpoint combinator
-   in [Equations] definitions. However, we need to take care that before 
-   applying the fixpoint combinator to an object in an inductive family,
-   we must first package it in a dependent sum. Consider the following 
-   programming problem: *)
+   in [Equations] definitions, we just need to deal with the currying when
+   applying it to an object in an inductive family. Consider the application 
+   of the fixpoint combinator for [vlast] again, our initial problem was: [[
+   forall A n (v : vector A (S n)), vlast_comp A n v]]
 
-Definition vlast_comp A n (v : vector A (S n)) := A.
+   To apply our recursion operator over vectors, we must first prepare 
+   for a dependent elimination on [v] packed with its index [n].
+   To do so, we simply generalize by an equality between the packed object 
+   and a fresh variable of the packed type, giving us an equivalent goal: *) 
 (* begin hide *)
+Definition vlast_comp A n (v : vector A (S n)) := A.
 Ltac fix_wf x recname := rec_wf_eqns x recname ; unfold add_pattern ;
   destruct_exists ; simpl in *; reverse ; simplify_dep_elim ; 
     repeat curry recname ; simpl in recname.
 Check projT1. Check projT2. Check nat. Check vector_subterm.
 Implicit Arguments existT [ [A] [P] ].
-(* end hide *)
+
 Definition vlast A n (v : vector A (S n)) : vlast_comp A n v.
 
 Proof.
-  (** To apply our recursion operator over vectors, we must first prepare 
-     for a dependent elimination on [v] packed with its index [n].
-     To do so, we simply generalize by an equality between the packed object 
-     and a fresh variable of the packed type, giving us an equivalent goal: *)
+(* end hide *)
   dependent generalize v as v'. simpl in *. revert_until v'.
   (* generalize_eqs_vars v. pack v as v'. clearbody v'. clear. intros n v0. *)
   (** [[
-(A : Type) (v' : {index : nat & vector A index})
+A : Type  v' : {index : nat & vector A index}
 ============================
 forall n (v : vector A (S n)), v' = existT (S n) v -> vlast_comp A n v ]]
    We can now directly use the fixpoint combinator on the 
-   subterm relation for packed vectors. This results in a new goal with 
+   subterm relation for packed vectors with [v']. This results in a new goal with 
    an additional induction hypothesis expecting a packed vector and 
-   a proof that it is smaller than the initial packed [v]. Using currying and 
-   unpacking of existentials, we get back a goal refining the initial 
-   problem. *)  
+   a proof that it is smaller than the initial packed [v]. Using currying, 
+   unpacking of existentials and the dependent elimination simplification tactic,
+   we get back a goal refining the initial problem with the same patterns [A n v]. *)  
   fix_wf v' rv.
   assert(forall (n' : nat) (v' : vector A (S n')),
     forall (index : nat) (y : vector A index),
@@ -76,20 +82,18 @@ forall n (v : vector A (S n)), v' = existT (S n) v -> vlast_comp A n v ]]
        @existT _ (fun n => vector A n) index y = existT (S n') v' -> vlast_comp A n' v').
   intros. apply rv with index y. auto. apply H0.
   simplify_IH_hyps. simpl in X.
-  
-
-  (** [[
+  (* [[
 (A : Type) (n : nat) (v : vector A (S n))
 recv : forall index y, vector_subterm A (existT index y) (existT (S n) v) ->
   forall n v, existT index y = existT (S n) v -> vlast_comp A n v
 ============================
- vlast_comp A n v ]]
- We can then continue our refinement and do recursive calls.
+ vlast_comp A n v ]] *)
+(** 
 
- The last step is to provide a proof search procedure to
+   The last step is to provide a proof search procedure to
  automatically build proofs of the subterm relation,
- filling the witnesses that appear at recursive calls (i.e. the 
- [vector_subterm] hypothesis here). We can easily do so using
+ filling the witnesses that appear at recursive calls.
+ We can easily do so using
  a hint database with the constructors of the $\ind{I}^{sub}$ 
  relation and lemmas on the transitive closure relation 
  that only allow to use the direct subterm relation on the right
@@ -98,4 +102,6 @@ recv : forall index y, vector_subterm A (existT index y) (existT (S n) v) ->
   depelim v. depelim v. exact a.
   change (vlast_comp A n (Vcons a0 v)).
   apply (rv (S n) (Vcons a0 v)) ; typeclasses eauto with subterm_relation Below.
+(* begin hide *)
 Defined.
+(* end hide *)
